Stated the better accountable safety

DynamicValidatorSet.thy
@@ -212,7 +212,6 @@ text "In a situation, a validator might be slashed or not.  A validator is slash
 although later we will be often talking ``unless one-third of the validators are slashed.''
 "
 
-(*
 text "[i] A validator is slashed when it has sent a commit message of a hash
       that is not prepared yet."
 
@@ -222,9 +221,7 @@ where
     (\<exists> h v.
       ((n, Commit (h, v)) \<in> Messages s \<and>
     (\<not> (\<exists> vs. -1 \<le> vs \<and> vs < v \<and> prepared s (RearValidators s h) h v vs) )))"
-*)
 
-(*
 text "[ii] A validator is slashed when it has sent a prepare message whose
       view src is not -1 but has no supporting preparation in the view src."
 
@@ -235,7 +232,6 @@ where
        ((n, Prepare (h, v, v_src)) \<in> Messages s \<and>
        v_src \<noteq> -1 \<and>
        (\<not> (\<exists> h_anc. sourcing s h_anc (h, v, v_src)))))"
-*)
 
 text "[iii] A validator is slashed when it has sent a commit message and a prepare message
      containing view numbers in a specific constellation."
@@ -1514,8 +1510,56 @@ lemma accountable_safety_for_legitimacy_fork :
    one_third_of_fwd_slashed s h'"
 using accountable_safety_center legitimacy_fork_with_center_and_root by blast
 
+section "Definitions Necessary for Accountable Safety (don't skip)"
+
+text "The above theorem only works for forks whose branches are made of the chain of sourcing.
+We are now going to turn any forks into such legitimacy forks.  A fork is simply three
+hashes that form a forking shape.
+"
+
+definition ancestor_descendant :: "situation \<Rightarrow> hash \<Rightarrow> hash \<Rightarrow> bool"
+where
+"ancestor_descendant s x y = (\<exists> n. nth_ancestor s n y = Some x)"
+
+definition on_same_chain :: "situation \<Rightarrow> hash \<Rightarrow> hash \<Rightarrow> bool"
+where "on_same_chain s x y = (ancestor_descendant s x y \<or> ancestor_descendant s y x)"
+
+fun fork :: "situation \<Rightarrow>
+                    hash \<Rightarrow>
+                    hash \<Rightarrow>
+                    hash \<Rightarrow> bool"
+where
+"fork s root h1 h2 =
+  (\<not> on_same_chain s h1 h2 \<and> ancestor_descendant s root h1 \<and> ancestor_descendant s root h2)"
+
+fun fork_with_commits :: "situation \<Rightarrow> (hash \<times> view) \<Rightarrow> (hash \<times> view) \<Rightarrow> (hash \<times> view) \<Rightarrow> bool"
+where
+"fork_with_commits s (h, v) (h1, v1) (h2, v2) =
+   (fork s h h1 h2 \<and>
+    committed_by_both s h v \<and>
+    committed_by_both s h1 v1 \<and>
+    committed_by_both s h2 v2)"
+
+section "Turning Any Fork into Legitimacy-Fork"
+
+lemma fork_contains_legitimacy_fork :
+"validator_sets_finite s \<Longrightarrow>
+ fork_with_commits s (h, v) (h1, v1) (h2, v2) \<Longrightarrow>
+ legitimacy_fork_with_commits s (h, v) (h1, v1) (h2, v2) \<or>
+ (\<exists> h' v'.
+   heir s (h, v) (h', v') \<and>
+   one_third_of_fwd_slashed s h')"
+sorry
+
 section "Accountable Safety for Any Fork"
 
+lemma accountable_safety :
+"validator_sets_finite s \<Longrightarrow>
+ fork_with_commits s (h, v) (h1, v1) (h2, v2) \<Longrightarrow>
+ \<exists> h' v'.
+   heir s (h, v) (h', v') \<and>
+   one_third_of_fwd_slashed s h'"
+using accountable_safety_for_legitimacy_fork fork_contains_legitimacy_fork by blast
 
 
 end
